adjacent sc: remove admits 7/n
preparing some removing
once within_bounds is fixed

src/Config.fst
@@ -4,16 +4,23 @@ open FStar.Mul
 
 let nb_size_classes = 9sz
 
+// required for metadata_max values
+// such that nb_size_classes * page_size * metadata_max > max_int 32
+module A = Steel.Array
+let _ : squash (US.fits_u64)
+  = A.intro_fits_u64 ()
+let _ : squash (UP.fits (FStar.Int.max_int 64))
+  = A.intro_fits_ptrdiff64 ()
+
 inline_for_extraction noextract
 let metadata_max' = 131072UL
-
-module A = Steel.Array
-let _ : squash (US.fits_u64) = A.intro_fits_u64 ()
 
 let metadata_max =
   US.fits_u64_implies_fits (U32.v page_size * U64.v metadata_max' * US.v nb_size_classes);
   US.fits_u64_implies_fits (U64.v metadata_max');
   US.of_u64 metadata_max'
+
+let metadata_max_up_fits _ = ()
 
 let alg_null = US.v metadata_max + 1
 
